specs/lib/Spec.Lib.IntBuf.Lemmas.fsti
@@ -1,0 +1,232 @@
+module Spec.Lib.IntBuf.Lemmas
+
+open FStar.HyperStack
+open FStar.HyperStack.ST
+open Spec.Lib.IntTypes
+
+module LSeq = Spec.Lib.IntSeq
+open Spec.Lib.IntBuf
+
+val live_sub_lemma: #a:Type0 -> #len:size_t -> h:mem -> b:lbuffer a len -> start:size_t -> n:size_t{start + n <= len} -> Lemma
+			 (requires (live h b))
+			 (ensures (live h (sub b start n)))
+			 [SMTPat (live h (sub b start n))]
+
+val live_super_lemma: #a:Type0 -> #len:size_t -> h:mem -> b:lbuffer a len -> start:size_t -> n:size_t{start + n <= len} -> Lemma
+			 (requires (live h (sub b start n)))
+			 (ensures (live h b))
+			 [SMTPat (live h (sub b start n))]
+
+val disjoint_self_lemma: #a:Type0 -> #len:size_t -> b:lbuffer a len -> Lemma
+			 (requires (True))
+			 (ensures (~ (disjoint b b)))
+			 [SMTPat (disjoint b b)]
+
+val disjoint_sub_lemma1: #a1:Type0 -> #a2:Type0 -> #len1:size_t -> #len2:size_t -> b1:lbuffer a1 len1 -> b2:lbuffer a2 len2 -> start1:size_t -> n1:size_t{start1 + n1 <= len1} -> Lemma
+			 (requires (disjoint b1 b2))
+			 (ensures (disjoint (sub b1 start1 n1) b2 /\ disjoint b2 (sub b1 start1 n1)))
+			 [SMTPat (disjoint (sub b1 start1 n1) b2);
+			  SMTPat (disjoint b2 (sub b1 start1 n1))]
+
+val disjoint_sub_lemma2: #a:Type0 -> #len:size_t -> b:lbuffer a len -> start1:size_t -> n1:size_t{start1 + n1 <= len} -> start2:size_t -> n2:size_t{start2 + n2 <= len} -> Lemma
+			 (requires (start1 + n1 <= start2 \/ start2 + n2 <= start1))
+			 (ensures (disjoint (sub b start1 n1) (sub b start2 n2)))
+			 [SMTPat (disjoint (sub b start1 n1) (sub b start2 n2))]
+
+val as_lseq_sub_lemma: #a:Type0 -> #len:size_t -> h:mem -> b:lbuffer a len -> start:size_t -> n:size_t{start + n <= len} -> Lemma
+			 (requires (live h b))
+			 (ensures (as_lseq (sub b start n) h == LSeq.sub (as_lseq b h) start n))
+			 [SMTPat (as_lseq (sub b start n) h)]
+			 
+			 
+val preserves_live_lemma: #a:Type0 -> #len:size_t -> b:lbuffer a len -> h0:mem -> h1:mem -> Lemma
+			 (requires (preserves_live h0 h1 /\ live h0 b))
+			 (ensures  (live h1 b))
+			 [SMTPat (preserves_live h0 h1);
+			  SMTPat (live h0 b)]
+
+
+val creates1_lemma:  #a1:Type0 -> #a2:Type0 -> #len1:size_t -> #len2:size_t -> b1:lbuffer a1 len1 -> b2:lbuffer a2 len2 -> h0:mem -> h1:mem -> Lemma
+			 (requires (live h0 b1 /\ creates1 b2 h0 h1))
+			 (ensures  (live h1 b1 /\ disjoint b1 b2 /\ disjoint b2 b1))
+			 [SMTPat (creates1 b2 h0 h1);
+			  SMTPat (live h0 b1)]
+
+val creates1_preserves:  #a1:Type0 -> #len1:size_t -> b:lbuffer a1 len1 -> h0:mem -> h1:mem -> h2:mem -> Lemma
+			 (requires (preserves_live h0 h1 /\ creates1 b h1 h2))
+			 (ensures  (creates1 b h0 h1))
+			 [SMTPat (creates1 b h1 h2);
+			  SMTPat (preserves_live h0 h1)]
+
+val creates1_preserves':  #a1:Type0 -> #len1:size_t -> b:lbuffer a1 len1 -> h0:mem -> h1:mem -> h2:mem -> Lemma
+			 (requires (creates1 b h0 h1 /\ preserves_live h1 h2))
+			 (ensures  (creates1 b h0 h2))
+			 [SMTPat (creates1 b h0 h1);
+			  SMTPat (preserves_live h1 h2)]
+
+let creates2 #a1 #a2 #len1 #len2 (b1:lbuffer a1 len1) (b2:lbuffer a2 len2) h0 h1 = 
+  creates1 #a1 #len1 b1 h0 h1 /\
+  creates1 #a2 #len2 b2 h0 h1 
+
+let creates3 #a1 #a2 #a3  #len1 #len2  #len3 (b1:lbuffer a1 len1) (b2:lbuffer a2 len2) (b3:lbuffer a3 len3) h0 h1 = 
+  creates1 #a1 #len1 b1 h0 h1 /\
+  creates1 #a2 #len2 b2 h0 h1 /\
+  creates1 #a3 #len3 b3 h0 h1 
+
+val live_list_lemma1: #a:Type0 -> #len:size_t -> b:lbuffer a len -> h:mem -> Lemma
+			(requires (True))
+			(ensures (live_list h [BufItem b] == live h b))
+			[SMTPat (live_list h [BufItem b])]
+
+val live_list_lemma2: #a1:Type0 -> #a2:Type0 -> #len1:size_t -> #len2:size_t -> b1:lbuffer a1 len1 -> b2:lbuffer a2 len2 -> h:mem -> Lemma
+			(requires (True))
+			(ensures (live_list h [BufItem b1; BufItem b2] == (live h b1 /\ live h b2)))
+			[SMTPat (live_list h [BufItem b1; BufItem b2])]
+
+val live_list_lemma3: #a1:Type0 -> #a2:Type0 -> #a3:Type0 -> #len1:size_t -> #len2:size_t -> #len3:size_t -> 
+			b1:lbuffer a1 len1 -> b2:lbuffer a2 len2 -> b3:lbuffer a3 len3 -> h:mem -> Lemma
+			(requires (True))
+			(ensures (live_list h [BufItem b1; BufItem b2; BufItem b3] == (live h b1 /\ live h b2 /\ live h b3)))
+			[SMTPat (live_list h [BufItem b1; BufItem b2; BufItem b3])]
+
+
+val disjoint_list_lemma1: #a:Type0 -> #a1:Type0 -> #len:size_t -> #len1:size_t -> b0:lbuffer a len -> b:lbuffer a len -> Lemma
+			(requires (True))
+			(ensures (disjoint_list b0 [BufItem b] == (disjoint b0 b /\ disjoint b b0) ))
+			[SMTPat (disjoint_list b0 [BufItem b])]
+
+val disjoint_list_lemma2: #a0:Type0 -> #a1:Type0 -> #a2:Type0 -> #len0:size_t -> #len1:size_t -> #len2:size_t -> b0:lbuffer a0 len0 -> b1:lbuffer a1 len1 -> b2:lbuffer a2 len2 ->  Lemma
+			(requires (True))
+			(ensures (disjoint_list b0 [BufItem b1; BufItem b2] == (disjoint b0 b1 /\ disjoint b0 b2 /\ disjoint b1 b0 /\ disjoint b2 b0)))
+			[SMTPat (disjoint_list b0 [BufItem b1; BufItem b2])]
+
+val disjoint_list_lemma3: #a0:Type0 -> #a1:Type0 -> #a2:Type0 -> #a3:Type0 -> #len0:size_t -> #len1:size_t -> #len2:size_t -> #len3:size_t -> 
+			b0:lbuffer a0 len0 -> b1:lbuffer a1 len1 -> b2:lbuffer a2 len2 -> b3:lbuffer a3 len3 -> Lemma
+			(requires (True))
+			(ensures (disjoint_list b0 [BufItem b1; BufItem b2; BufItem b3] == (disjoint b0 b1 /\ disjoint b0 b2 /\ disjoint b0 b3 /\ disjoint b1 b0 /\ disjoint b2 b0 /\ disjoint b3 b0)))
+			[SMTPat (disjoint_list b0 [BufItem b1; BufItem b2; BufItem b3])]
+
+val modifies_modifies_1: #a:Type0 -> #len:size_t -> b:lbuffer a len -> h0:mem -> h1:mem -> Lemma
+			(requires (True))
+			(ensures (modifies [BufItem b] h0 h1 == modifies1 b h0 h1))
+			[SMTPat (modifies [BufItem b] h0 h1)]
+
+val list_cons1_lemma: #a:Type0 -> x:a -> y:a -> Lemma
+			 (requires True)
+			 (ensures ([x;y] == x::[y]))
+			 [SMTPat (x::[y])]
+val list_cons2_lemma: #a:Type0 -> x:a -> y:a -> z:a -> Lemma
+			 (requires True)
+			 (ensures ([x;y;z] == x::[y;z]))
+			 [SMTPat (x::[y;z])]
+			 
+val modifies_modifies_2: #a1:Type0 -> #a2:Type0 -> #len1:size_t -> #len2:size_t -> 
+			b1:lbuffer a1 len1 -> b2:lbuffer a2 len2 -> h0:mem -> h1:mem -> Lemma
+			(requires (True))
+			(ensures (modifies [BufItem b1; BufItem b2] h0 h1 == modifies2 b1 b2 h0 h1))
+			[SMTPat (modifies [BufItem b1; BufItem b2] h0 h1)]
+
+val modifies_modifies_3: #a1:Type0 -> #a2:Type0 -> #a3:Type0 -> #len1:size_t -> #len2:size_t -> #len3:size_t -> 
+			b1:lbuffer a1 len1 -> b2:lbuffer a2 len2 -> b3:lbuffer a3 len3 -> 
+			h0:mem -> h1:mem -> Lemma
+			(requires True) 
+			(ensures (modifies [BufItem b1; BufItem b2; BufItem b3] h0 h1 == modifies3 b1 b2 b3 h0 h1))
+			[SMTPat (modifies [BufItem b1; BufItem b2; BufItem b3] h0 h1)]
+
+val preserves_live_refl: h0:mem -> Lemma
+		         (requires (True))
+			 (ensures (preserves_live h0 h0))
+			 [SMTPat (preserves_live h0 h0)]
+
+val preserves_live_trans: h0:mem -> h1:mem -> h2:mem -> Lemma
+		         (requires (preserves_live h0 h1 /\ preserves_live h1 h2))
+			 (ensures (preserves_live h0 h2))
+			 [SMTPat (preserves_live h0 h1);
+			  SMTPat (preserves_live h1 h2)]
+
+val modifies_1_refl: #a:Type0 -> #len:size_t -> b:lbuffer a len -> h0:mem -> Lemma
+			 (requires (live h0 b))
+			 (ensures (modifies1 b h0 h0))
+			 [SMTPat (modifies1 b h0 h0)]
+
+val modifies_1_modifies_2: #a1:Type0 -> #a2:Type0 -> #len1:size_t -> #len2:size_t -> b1:lbuffer a1 len1 -> b2:lbuffer a2 len2 -> h0:mem -> h1:mem -> Lemma
+			 (requires (live h0 b1 /\ live h0 b2 /\ modifies1 b1 h0 h1))
+			 (ensures (modifies2 b1 b2 h0 h1 /\ modifies2 b2 b1 h0 h1))
+			 [SMTPat (modifies1 b1 h0 h1);
+			  SMTPat (live h0 b1);
+			  SMTPat (live h0 b2)]
+
+
+val modifies_2_modifies_3: #a1:Type0 -> #a2:Type0 -> #a3:Type0 -> #len1:size_t -> #len2:size_t -> #len3:size_t -> 
+		           b1:lbuffer a1 len1 -> b2:lbuffer a2 len2 -> b3:lbuffer a3 len3 -> h0:mem -> h1:mem -> Lemma
+			 (requires (live h0 b1 /\ live h0 b2 /\ live h0 b3 /\ modifies2 b1 b2 h0 h1))
+			 (ensures (modifies3 b1 b2 b3 h0 h1 /\ modifies3 b1 b3 b2 h0 h1 /\ modifies3 b2 b1 b3 h0 h1 /\ 
+				   modifies3 b2 b3 b1 h0 h1 /\ modifies3 b3 b1 b2 h0 h1 /\ modifies3 b3 b2 b1 h0 h1))
+			 [SMTPat (modifies2 b1 b2 h0 h1);
+			  SMTPat (live h0 b1);
+			  SMTPat (live h0 b2);
+			  SMTPat (live h0 b3)]
+
+
+val modifies_1_trans: #a:Type0 -> #len:size_t -> b:lbuffer a len -> h0:mem -> h1:mem -> h2:mem -> Lemma
+			 (requires (live h0 b /\ modifies1 b h0 h1 /\ modifies1 b h1 h2))
+			 (ensures (modifies1 b h0 h2))
+			 [SMTPat (modifies1 b h0 h1);
+			  SMTPat (modifies1 b h1 h2);
+			  SMTPat (live h0 b)]
+
+
+val modifies_2_trans: #a1:Type0 -> #a2:Type0 -> #len1:size_t -> #len2:size_t -> b1:lbuffer a1 len1 -> b2:lbuffer a2 len2 -> h0:mem -> h1:mem -> h2:mem -> Lemma
+			 (requires (live h0 b1 /\ live h0 b2 /\ modifies2 b1 b2 h0 h1 /\ modifies2 b1 b2 h1 h2))
+			 (ensures (modifies2 b1 b2 h0 h2))
+			 [SMTPat (modifies2 b1 b2 h0 h1);
+			  SMTPat (modifies2 b1 b2 h1 h2);
+			  SMTPat (live h0 b1);
+			  SMTPat (live h0 b2)]
+
+val modifies_3_trans: #a1:Type0 -> #a2:Type0 -> #a3:Type0 -> #len1:size_t -> #len2:size_t -> #len3:size_t -> 
+		           b1:lbuffer a1 len1 -> b2:lbuffer a2 len2 -> b3:lbuffer a3 len3 -> h0:mem -> h1:mem -> h2:mem -> Lemma
+			 (requires (live h0 b1 /\ live h0 b2 /\ live h0 b3 /\ modifies3 b1 b2 b3 h0 h1 /\ modifies3 b1 b2 b3 h1 h2))
+			 (ensures (modifies3 b1 b2 b3 h0 h2))
+			 [SMTPat (modifies3 b1 b2 b3 h0 h1);
+			  SMTPat (modifies3 b1 b2 b3 h1 h2);
+			  SMTPat (live h0 b1);
+			  SMTPat (live h0 b2);
+			  SMTPat (live h0 b3)]
+
+
+val modifies1_lemma:  #a1:Type0 -> #a2:Type0 -> #len1:size_t -> #len2:size_t -> b1:lbuffer a1 len1 -> b2:lbuffer a2 len2 -> h0:mem -> h1:mem -> Lemma
+			 (requires (disjoint b1 b2 /\ live h0 b1 /\ modifies1 b2 h0 h1))
+			 (ensures  (live h1 b1 /\ as_lseq b1 h1 == as_lseq b1 h0))
+			 [SMTPat (disjoint b1 b2);
+			  SMTPat (live h0 b1);
+			  SMTPat (modifies1 b2 h0 h1)]
+
+
+val modifies2_lemma:  #a1:Type0 -> #a2:Type0 -> #a3:Type0 -> #len1:size_t -> #len2:size_t -> #len3:size_t -> b1:lbuffer a1 len1 -> b2:lbuffer a2 len2 -> b3:lbuffer a3 len3 -> h0:mem -> h1:mem -> Lemma
+			 (requires (disjoint b1 b2 /\ disjoint b1 b3 /\ live h0 b1 /\ modifies2 b2 b3 h0 h1))
+			 (ensures  (live h1 b1 /\ as_lseq b1 h1 == as_lseq b1 h0))
+			 [SMTPat (disjoint b1 b2);
+			  SMTPat (disjoint b1 b3);
+			  SMTPat (live h0 b1);
+			  SMTPat (modifies2 b2 b3 h0 h1)]
+
+
+val modifies3_lemma:  #a1:Type0 -> #a2:Type0 -> #a3:Type0 -> #a4:Type0-> #len1:size_t -> #len2:size_t -> #len3:size_t -> #len4:size_t -> 
+		      b1:lbuffer a1 len1 -> b2:lbuffer a2 len2 -> b3:lbuffer a3 len3 -> b4:lbuffer a4 len4 -> h0:mem -> h1:mem -> Lemma
+			 (requires (disjoint b1 b2 /\ disjoint b1 b3 /\ disjoint b1 b4 /\ live h0 b1 /\ modifies3 b2 b3 b4 h0 h1))
+			 (ensures  (live h1 b1 /\ as_lseq b1 h1 == as_lseq b1 h0))
+			 [SMTPat (disjoint b1 b2);
+			  SMTPat (disjoint b1 b3);
+			  SMTPat (disjoint b1 b4);
+			  SMTPat (live h0 b1);
+			  SMTPat (modifies3 b2 b3 b4 h0 h1)]
+
+
+val modifies_sub_lemma: #a:Type0 -> #len:size_t -> b:lbuffer a len -> start:size_t -> n:size_t{start+n <= len} -> h0:mem -> h1:mem -> Lemma
+			 (requires (live h0 b /\ modifies1 (sub b start n) h0 h1))
+			 (ensures  (modifies1 b h0 h1 /\ as_lseq b h1 == LSeq.update_sub (as_lseq b h0) start n (LSeq.sub (as_lseq b h1) start n)))
+			 [SMTPat (live h0 b);
+			  SMTPat (modifies1 (sub b start n) h0 h1)]
+
+
