specs/lib/Spec.Lib.IntSeq.fsti
@@ -69,3 +69,9 @@ val uints_from_bytes_be: #t:inttype -> #len:size_t{len `op_Multiply` numbytes t 
 //The following function is primarily meant for testing, do not rely on it in code.
 val as_list: #a:Type -> #len:size_t -> lseq a len -> l:list a{List.Tot.length l = len}
 
+val map_block: #a:Type -> #b:Type -> n:size_t -> 
+		blocksize:size_t{n `op_Multiply` blocksize <= max_size_t} -> 
+		(i:size_t{i < n} -> lseq a blocksize -> lseq b blocksize) -> 
+		lseq a (n `op_Multiply` blocksize) -> 
+		Tot (lseq b (n `op_Multiply` blocksize))
+
